src/lang/Configuration.v
@@ -1,0 +1,95 @@
+Require Import Omega.
+
+Require Import sflib.
+
+Require Import Basic.
+Require Import DataStructure.
+Require Import Time.
+Require Import Event.
+Require Import Thread.
+Require Import Memory.
+
+Set Implicit Arguments.
+
+
+Module Context.
+  Structure t := mk {
+    thread: Thread.t;
+    local: ThreadLocal.t;
+    memory: Memory.t;
+  }.
+
+  Inductive step (ctx1:t): forall (ctx2:t), Prop :=
+  | step_local
+      th2 thl2
+      (THREAD: Thread.step ctx1.(thread) None th2)
+      (COMMIT: ThreadLocal.step ctx1.(local) thl2):
+      step ctx1 (mk th2 thl2 ctx1.(memory))
+  | step_mem
+      e th2 thl2
+      (THREAD: Thread.step ctx1.(thread) (Some (ThreadEvent.mem e)) th2)
+      (MEM: Memory.step ctx1.(local) ctx1.(memory) e thl2):
+      step ctx1 (mk th2 thl2 ctx1.(memory))
+  | step_declare
+      thl2 mem2
+      (MEM: Memory.declare ctx1.(local) ctx1.(memory) thl2 mem2):
+      step ctx1 (mk ctx1.(thread) thl2 mem2)
+  .
+End Context.
+
+Module Configuration.
+  Definition syntax := IdentMap.t Thread.syntax.
+
+  Structure t := mk {
+    threads: IdentMap.t (Thread.t * ThreadLocal.t);
+    memory: Memory.t;
+  }.
+
+  Definition init (s:syntax): t :=
+    mk (IdentMap.map (fun th => (Thread.init th, ThreadLocal.init)) s)
+       Memory.init.
+
+  Definition is_terminal (conf:t): Prop :=
+    forall tid th thl (FIND: IdentMap.find tid conf.(threads) = Some (th, thl)),
+      Thread.is_terminal th.
+
+  Inductive internal_step (c1:t): forall (c2:t), Prop :=
+  | internal_step_intro
+      tid th1 thl1 th2 thl2 memory2
+      (FIND: IdentMap.find tid c1.(threads) = Some (th1, thl1))
+      (STEP: tc Context.step (Context.mk th1 thl1 c1.(memory)) (Context.mk th2 thl2 memory2)):
+      internal_step c1 (mk (IdentMap.add tid (th2, thl2) c1.(threads)) memory2)
+  .
+
+  Inductive external_step (c1:t): forall (e:Event.t) (c2:t), Prop :=
+  | external_step_intro
+      tid th1 thl1 th2 thl2 e
+      (FIND: IdentMap.find tid c1.(threads) = Some (th1, thl1))
+      (THREAD: Thread.step th1 (Some (ThreadEvent.syscall e)) th2):
+      external_step
+        c1 e
+        (mk (IdentMap.add tid (th2, thl2) c1.(threads)) c1.(memory))
+  .
+
+  Definition consistent (conf:t): Prop :=
+    forall tid th thl mem_future
+      (FIND: IdentMap.find tid conf.(threads) = Some (th, thl))
+      (FUTURE: Memory.future thl.(ThreadLocal.permission) conf.(memory) mem_future),
+    exists th' thl' mem_future',
+      <<STEPS: rtc Context.step (Context.mk th thl mem_future) (Context.mk th' thl' mem_future')>> /\
+      <<NODECLAURE: thl'.(ThreadLocal.declares) = DeclareSet.empty>>.
+
+  Inductive step: forall (c1:t) (e:option Event.t) (c2:t), Prop :=
+  | step_internal
+      c1 c2
+      (STEP: internal_step c1 c2)
+      (CONSISTENT: consistent c2):
+      step c1 None c2
+  | step_external
+      c1 c2
+      e
+      (STEP: external_step c1 e c2)
+      (CONSISTENT: consistent c2):
+      step c1 (Some e) c2
+  .
+End Configuration.
