src/lang/Memory.v
@@ -1,0 +1,260 @@
+Require Import Omega.
+
+Require Import sflib.
+
+Require Import Basic.
+Require Import DataStructure.
+Require Import Time.
+Require Import Event.
+
+Set Implicit Arguments.
+
+Module Timestamps.
+  Definition t := LocFun.t Time.t.
+  Definition init: t := LocFun.init Time.elt.
+
+  Definition le (lhs rhs:t): Prop :=
+    forall loc, Time.le (LocFun.find loc lhs) (LocFun.find loc rhs).
+
+  Definition get (loc:Loc.t) (c:t) :=
+    LocFun.find loc c.
+End Timestamps.
+
+Module History.
+  Structure t := mk {
+    reads: Timestamps.t;
+    writes: Timestamps.t;
+  }.
+
+  Definition init: t := mk Timestamps.init Timestamps.init.
+
+  Inductive le (lhs rhs:t): Prop :=
+  | le_intro
+      (READS: Timestamps.le lhs.(reads) rhs.(reads))
+      (WRITES: Timestamps.le lhs.(writes) rhs.(writes))
+  .
+
+  Inductive readable (history:t) (loc:Loc.t) (ts:Time.t): Prop :=
+  | readable_intro
+      (* (CoRR: Time.le (Timestamps.get loc history.(History.reads)) ts) *)
+      (CoWR: Time.le (Timestamps.get loc history.(History.writes)) ts)
+  .
+
+  Inductive writable (history:t) (loc:Loc.t) (ts:Time.t): Prop :=
+  | writable_intro
+      (CoRW: Time.lt (Timestamps.get loc history.(History.reads)) ts)
+      (CoWW: Time.lt (Timestamps.get loc history.(History.writes)) ts)
+  .
+End History.
+
+Module Commit.
+  Structure t := mk {
+    current: History.t;
+    released: LocFun.t History.t;
+    acquirable: History.t;
+  }.
+
+  Definition init: t := mk History.init (LocFun.init History.init) History.init.
+
+  Inductive le (lhs rhs:t): Prop :=
+  | le_intro
+      (CURRENT: History.le lhs.(current) rhs.(current))
+      (RELEASED: forall (loc:Loc.t), History.le (LocFun.find loc lhs.(released)) (LocFun.find loc rhs.(released)))
+      (ACQUIRABLE: History.le lhs.(acquirable) rhs.(acquirable))
+  .
+
+  Inductive read
+            (commit1:t) (loc:Loc.t) (ts:Time.t) (released:History.t) (ord:Ordering.t)
+            (commit2:t): Prop :=
+  | read_intro
+      (FUTURE: le commit1 commit2)
+      (READABLE: History.readable commit1.(current) loc ts)
+      (READ: Time.le ts (Timestamps.get loc commit2.(current).(History.reads)))
+      (ACQUIRE: forall (ORDERING: Ordering.le Ordering.acquire ord),
+          History.le released commit2.(current))
+      (ACQUIRABLE: History.le released commit2.(acquirable))
+  .
+
+  Inductive write
+            (commit1:t) (loc:Loc.t) (ts:Time.t) (released:History.t) (ord:Ordering.t)
+            (commit2:t): Prop :=
+  | write_intro
+      (FUTURE: le commit1 commit2)
+      (WRITABLE: History.writable commit1.(current) loc ts)
+      (WRITE: Time.le ts (Timestamps.get loc commit2.(current).(History.writes)))
+      (RELEASE: forall (ORDERING: Ordering.le Ordering.release ord),
+          History.le commit2.(current) released)
+      (RELEASED: History.le (LocFun.find loc commit2.(Commit.released)) released)
+  .
+
+  Inductive fence
+            (commit1:t) (ord:Ordering.t)
+            (commit2:t): Prop :=
+  | fence_intro
+      (FUTURE: le commit1 commit2)
+      (ACQUIRE: forall (ORDERING: Ordering.le Ordering.acquire ord),
+          History.le commit2.(acquirable) commit2.(current))
+      (RELEASE: forall (ORDERING: Ordering.le Ordering.release ord) loc,
+          History.le commit2.(current) (LocFun.find loc commit2.(released)))
+  .
+End Commit.
+
+Module Permission.
+  Definition t := LocFun.t IntervalSet.t.
+  Definition bot: t := LocFun.init IntervalSet.empty.
+
+  Definition has_perm (loc:Loc.t) (ts:Time.t) (perm:t): Prop :=
+    IntervalSet.time_mem ts (LocFun.find loc perm).
+
+  Definition disjoint (lhs rhs:t): Prop :=
+    forall loc, IntervalSet.time_disjoint (LocFun.find loc lhs) (LocFun.find loc rhs).
+
+  Definition le (lhs rhs:t): Prop :=
+    forall loc ts (LHS: IntervalSet.time_mem ts (LocFun.find loc lhs)),
+      IntervalSet.time_mem ts (LocFun.find loc rhs).
+
+  Definition add (loc:Loc.t) (ts0 ts:Time.t) (perm:t): t :=
+    LocFun.add loc (IntervalSet.add (ts0, ts) (LocFun.find loc perm)) perm.
+End Permission.
+
+Module DeclareSet.
+  Definition t := LocFun.t TimeSet.t.
+  Definition empty: t := LocFun.init TimeSet.empty.
+
+	Definition get loc ts (ds:t): bool :=
+    TimeSet.mem ts (LocFun.find loc ds).
+
+	Definition set loc ts (ds:t): t :=
+    LocFun.add loc (TimeSet.add ts (LocFun.find loc ds)) ds.
+
+	Definition unset loc ts (ds:t): t :=
+    LocFun.add loc (TimeSet.remove ts (LocFun.find loc ds)) ds.
+
+	Definition add loc ts (ds:t): option t :=
+    if get loc ts ds
+    then None
+    else Some (set loc ts ds).
+
+	Definition remove loc ts (ds:t): option t :=
+    if get loc ts ds
+    then Some (unset loc ts ds)
+    else None.
+End DeclareSet.
+
+Module ThreadLocal.
+  Structure t := mk {
+    commit: Commit.t;
+    permission: Permission.t;
+    declares: DeclareSet.t;
+  }.
+
+  Definition init := mk Commit.init Permission.bot DeclareSet.empty.
+
+  Inductive step (lhs rhs:t): Prop :=
+  | step_intro
+      (COMMIT: Commit.le lhs.(commit) rhs.(commit))
+      (PERMISSION: lhs.(permission) = rhs.(permission))
+      (DECLARES: lhs.(declares) = rhs.(declares))
+  .
+End ThreadLocal.
+
+
+Module Message.
+  Structure t := mk {
+    val: Const.t;
+    released: History.t;
+  }.
+
+  Inductive future: forall (lhs rhs:option t), Prop :=
+  | future_None rhs:
+      future None rhs
+  | future_Some msg:
+      future (Some msg) (Some msg)
+  .
+End Message.
+
+Module Memory.
+  Structure t := mk {
+    messages: LocFun.t (TimeFun.t (option Message.t));
+    permission: Permission.t;
+  }.
+
+  Definition init: t :=
+    mk (LocFun.init (TimeFun.add Time.elt (Some (Message.mk 0 History.init)) (TimeFun.init None)))
+       Permission.bot.
+
+  Definition get (loc:Loc.t) (ts:Time.t) (m:t): option Message.t :=
+    TimeFun.find ts (LocFun.find loc m.(messages)).
+
+  Definition set (loc:Loc.t) (ts:Time.t) (msg:Message.t) (m:t): t :=
+    mk (LocFun.add loc (TimeFun.add ts (Some msg) (LocFun.find loc m.(messages))) m.(messages))
+       m.(permission).
+
+  Inductive add (perm:Permission.t) (loc:Loc.t) (ts0 ts:Time.t) (msg:Message.t) (lhs:t): forall (rhs:t), Prop :=
+  | add_intro
+      (PERM: forall x
+               (ITV: Interval.time_mem x (ts0, ts))
+               (MEM: Permission.has_perm loc x lhs.(permission)),
+          Permission.has_perm loc x perm)
+      (LHS: get loc ts lhs = None):
+      add perm loc ts0 ts msg lhs (set loc ts msg lhs)
+  .
+
+  Inductive step (thl1:ThreadLocal.t) (mem1:t): forall (e:MemEvent.t) (thl2:ThreadLocal.t), Prop :=
+  | step_read
+      loc val ts released ord commit2
+      (COMMIT: Commit.read thl1.(ThreadLocal.commit) loc ts released ord commit2)
+      (DECLARES: DeclareSet.get loc ts thl1.(ThreadLocal.declares) = false)
+      (MEMORY: get loc ts mem1 = Some (Message.mk val released)):
+      step thl1 mem1 (MemEvent.read loc val ord)
+           (ThreadLocal.mk commit2 thl1.(ThreadLocal.permission) thl1.(ThreadLocal.declares))
+  | step_write
+      loc val ts released ord commit2 declares2
+      (COMMIT: Commit.write thl1.(ThreadLocal.commit) loc ts released ord commit2)
+      (PERMISSION: Permission.has_perm loc ts thl1.(ThreadLocal.permission))
+      (DECLARES: DeclareSet.remove loc ts thl1.(ThreadLocal.declares) = Some declares2)
+      (MEMORY: get loc ts mem1 = Some (Message.mk val released)):
+      step thl1 mem1
+           (MemEvent.write loc val ord)
+           (ThreadLocal.mk commit2 thl1.(ThreadLocal.permission) declares2)
+  | step_update
+      loc valr tsr releasedr valw tsw releasedw ord commit2 commit3 declares3
+      (COMMIT1: Commit.read thl1.(ThreadLocal.commit) loc tsr releasedr ord commit2)
+      (COMMIT2: Commit.write commit2 loc tsw releasedw ord commit3)
+      (RELEASED: History.le releasedr releasedw)
+      (PERMISSION: forall x (ITV: Interval.time_mem x (tsr, tsw)), IntervalSet.time_mem x (LocFun.find loc thl1.(ThreadLocal.permission)))
+      (DECLARES: DeclareSet.remove loc tsw thl1.(ThreadLocal.declares) = Some declares3)
+      (MEMORY1: get loc tsr mem1 = Some (Message.mk valr releasedr))
+      (MEMORY2: get loc tsw mem1 = Some (Message.mk valw releasedw)):
+      step thl1 mem1
+           (MemEvent.update loc valr valw ord)
+           (ThreadLocal.mk commit3 thl1.(ThreadLocal.permission) declares3)
+  | step_fence
+      ord commit2
+      (COMMIT: Commit.fence thl1.(ThreadLocal.commit) ord commit2):
+      step thl1 mem1
+           (MemEvent.fence ord)
+           (ThreadLocal.mk commit2 thl1.(ThreadLocal.permission) thl1.(ThreadLocal.declares))
+  .
+
+  Inductive declare (thl1:ThreadLocal.t) (mem1:t): forall (thl2:ThreadLocal.t) (mem2:t), Prop :=
+  | declare_intro
+      loc ts val released ts0 thl2
+      (TS: Time.le ts0 ts)
+      (COMMIT: Commit.le thl1.(ThreadLocal.commit) thl2.(ThreadLocal.commit))
+      (PERMISSION: Permission.add loc ts0 ts thl1.(ThreadLocal.permission) = thl2.(ThreadLocal.permission))
+      (DECLARE: DeclareSet.add loc ts thl1.(ThreadLocal.declares) = Some thl2.(ThreadLocal.declares))
+      (PERM: forall x (ITV: Interval.time_mem x (ts0, ts)) (MEM: Permission.has_perm loc x mem1.(permission)),
+          Permission.has_perm loc x thl1.(ThreadLocal.permission))
+      (GET: get loc ts mem1 = None):
+      declare thl1 mem1 thl2 (set loc ts (Message.mk val released) mem1)
+  .
+
+  Inductive future (perm:Permission.t) (lhs rhs:t): Prop :=
+  | future_intro
+      (MESSAGE: forall loc ts, Message.future (get loc ts lhs) (get loc ts rhs))
+      (NONPERM: forall loc ts (NONPERM: Permission.has_perm loc ts perm),
+          get loc ts lhs = get loc ts rhs)
+      (PERM: Permission.le lhs.(permission) rhs.(permission))
+  .
+End Memory.
