src/lang/Time.v
@@ -1,0 +1,39 @@
+Require Import Orders.
+
+Require Import sflib.
+
+Require Import DataStructure.
+Require Import DenseOrder.
+
+Module Time := DenseOrder.
+
+Module Interval <: UsualOrderedType.
+  Include UsualProd Time Time.
+
+  Inductive time_mem (x:Time.t) (interval:t): Prop :=
+  | time_mem_intro
+      (FROM: Time.lt interval.(fst) x)
+      (TO: ~ Time.lt interval.(snd) x)
+  .
+End Interval.
+
+
+Module TimeSet := UsualSet Time.
+Module TimeFun := UsualFun Time.
+
+Module IntervalSet.
+  Include UsualSet Interval.
+
+  Inductive time_mem (x:Time.t) (intervals:t): Prop :=
+  | time_mem_intro
+      itv
+      (ITV: Interval.time_mem x itv)
+      (ITVS: mem itv intervals)
+  .
+
+  Definition time_disjoint (lhs rhs:t): Prop :=
+    forall x
+      (LHS: time_mem x lhs)
+      (RHS: time_mem x rhs),
+      False.
+End IntervalSet.
