src/lib/DenseOrder.v
@@ -1,0 +1,137 @@
+Require Import Orders.
+
+Require Import sflib.
+Require Import paco.
+
+Require Import Basic.
+Require Import DataStructure.
+
+Module Type HasMiddle (Import T:EqLt).
+  Parameter elt: t.
+
+  Axiom unbounded:
+    forall (x:t),
+    exists (y:t),
+      lt x y.
+
+  Parameter middle: forall (lhs rhs:t), t.
+  Axiom middle_spec:
+    forall (lhs rhs:t)
+      (LT: lt lhs rhs),
+      lt lhs (middle lhs rhs) /\
+      lt (middle lhs rhs) rhs.
+End HasMiddle.
+
+Module Type DenseOrderType := UsualOrderedTypeFull <+ HasMiddle.
+
+Module DenseOrder: DenseOrderType.
+  Definition t := list bool.
+  Definition elt: t := nil.
+
+  Definition eq := @eq t.
+  Global Program Instance eq_equiv : Equivalence eq.
+
+  Inductive lt_: forall (lhs rhs:t), Prop :=
+  | lt_false lhs:
+      lt_ (false::lhs) []
+  | lt_true rhs:
+      lt_ [] (true::rhs)
+  | lt_false_true lhs rhs:
+      lt_ (false::lhs) (true::rhs)
+  | lt_cons
+      hd lhs rhs
+      (LT: lt_ lhs rhs):
+      lt_ (hd::lhs) (hd::rhs)
+  .
+  Definition lt := lt_.
+  Global Program Instance lt_strorder: StrictOrder lt.
+  Next Obligation.
+    intro x. induction x; intro X; inv X.
+    apply IHx. auto.
+  Qed.
+  Next Obligation.
+    intros x y z XY. revert z.
+    induction XY; i; inv H; econs.
+    apply IHXY. auto.
+  Qed.
+  Global Program Instance lt_compat: Proper (eq ==> eq ==> iff) lt.
+  Next Obligation.
+    ii. unfold eq in *. subst. auto.
+  Qed.
+  Fixpoint compare (lhs rhs:t): comparison :=
+    match lhs, rhs with
+    | [], [] =>
+      Eq
+    | false::_, true::_
+    | [], true::_
+    | false::_, [] =>
+      Lt
+    | true::_, false::_
+    | [], false::_
+    | true::_, [] =>
+      Gt
+    | false::ltl, false::rtl
+    | true::ltl, true::rtl =>
+      compare ltl rtl
+    end.
+   Lemma compare_spec :
+     forall x y : t,
+       CompareSpec (x = y) (lt x y) (lt y x) (compare x y).
+   Proof.
+     induction x; i; destruct y;
+       try (destruct a);
+       try (destruct b);
+       repeat (try econs; simpl).
+     - destruct (IHx y); subst; repeat econs; auto.
+     - destruct (IHx y); subst; repeat econs; auto.
+   Qed.
+
+   Lemma eq_dec: forall x y : t, {x = y} + {x <> y}.
+   Proof.
+     induction x; destruct y.
+     - left. auto.
+     - right. congruence.
+     - right. congruence.
+     - destruct (IHx y).
+       + subst. destruct (Bool.eqb a b) eqn:HD.
+         * destruct a, b; auto.
+         * right. destruct a, b; inv HD; congruence.
+       + right. congruence.
+   Qed.
+
+   Definition le := lt \2/ eq.
+   Lemma le_lteq : forall x y : t, le x y <-> lt x y \/ x = y.
+   Proof. auto. Qed.
+
+   Lemma unbounded:
+     forall (x:t),
+     exists (y:t),
+       lt x y.
+   Proof.
+     i. exists (x ++ [true]). induction x; econs; auto.
+   Qed.
+
+   Fixpoint middle (lhs rhs:t): t :=
+     match lhs, rhs with
+     | [], rhs => rhs ++ [false]
+     | lhs, [] => lhs ++ [true]
+     | false::ltl, true::rtl => []
+     | lhd::ltl, rhd::rtl => lhd::(middle ltl rtl)
+     end.
+  Lemma middle_spec:
+    forall (lhs rhs:t)
+      (LT: lt lhs rhs),
+      lt lhs (middle lhs rhs) /\
+      lt (middle lhs rhs) rhs.
+  Proof.
+    induction lhs; i; inv LT; splits; try econs; simpl.
+    - induction rhs0; econs.
+      apply IHrhs0.
+    - clear IHlhs. induction lhs; econs.
+      apply IHlhs.
+    - exploit IHlhs; eauto. i. des.
+      destruct a; econs; auto.
+    - exploit IHlhs; eauto. i. des.
+      destruct a; econs; auto.
+  Qed.
+End DenseOrder.
